adding some automation

theories/Properties.v
@@ -5,106 +5,117 @@ From MetaCoq.PCUIC Require Export PCUICCumulativitySpec.
 From MetaCoq.PCUIC Require Export PCUICCases PCUICNormal.
 From LogRel Require Import MLTTTyping Untyped.
 
+Create HintDb mltt.
+#[global] Hint Constants Opaque : mltt.
+#[global] Hint Variables Transparent : mltt.
+
+Ltac mltt := eauto with mltt.
+
+#[global] Hint Constructors wfType wfContext wfTerm convType convTerm : mltt.
+#[global] Hint Constructors termRed typeRed : mltt.
+
+(*Making the non syntax-directed hints more costly*)
+#[global] Remove Hints wfTermConv TermConv termRedConv : mltt.
+#[global] Hint Resolve wfTermConv TermConv termRedConv | 10 : mltt.
+
+Definition concons_inv {Γ na A} : [|- Γ,, vass na A] -> [|- Γ].
+Proof.
+  now inversion 1.
+Qed.
+
+Definition concons_inv' {Γ na A} : [|- Γ,, vass na A] -> [Γ |- A].
+Proof.
+  now inversion 1.
+Qed.
+
+#[global] Hint Resolve concons_inv concons_inv': mltt.
+
 Definition WFterm {Γ} {t A} :
     [ Γ |- t ::: A ] -> 
     [ |- Γ ].
 Proof.
-    intros.
-    induction X; try assumption.
-    inversion IHX. assumption.
+  induction 1 ; mltt.
 Defined.
 
+#[global] Hint Resolve WFterm : mltt.
 
 Definition WFtype {Γ} {A} :
     [ Γ |- A ] -> 
     [ |- Γ ].
 Proof.
-    intros.
-    induction X; try assumption.
-    now eapply WFterm.
+    induction 1; mltt.
 Defined.
+
+#[global] Hint Resolve WFtype : mltt.
 
 Definition WFEqTerm {Γ} {t u A} :
     [ Γ |- t ≅ u ::: A ] -> 
     [ |- Γ ].
 Proof.
-    intros.
-    induction X; try assumption.
-    - exact (WFterm w).
-    - exact (WFterm w1).
-    - exact (WFterm w0).
+    induction 1; mltt.
 Defined.
+
+#[global] Hint Resolve WFEqTerm : mltt.
 
 Definition WFEqType {Γ} {A B} :
     [ Γ |- A ≅ B ] -> 
     [ |- Γ ].
 Proof.
-    intros.
-    induction X; try assumption.
-    1: destruct w; try eassumption.
-    - exact (WFtype w1).
-    - exact (WFterm w).
-    - exact (WFEqTerm c).
+  induction 1 ; mltt.
 Defined.
+
+#[global] Hint Resolve WFEqType : mltt.
 
 Definition redFirstTerm {Γ t u A} : 
   [ Γ |- t ⇒ u ::: A] ->
   [ Γ |- t ::: A ].
 Proof.
-  intros.
-  induction X.
-  - exact (wfTermConv IHX c).
-  - eapply wfTermApp; eassumption.
-  - eapply wfTermApp; try eassumption.
-    eapply wfTermLam; eassumption.
+  induction 1 ; mltt.
 Defined.
+
+#[global] Hint Resolve redFirstTerm : mltt.
 
 Definition redFirst {Γ A B} : 
   [ Γ |- A ⇒ B ] ->
   [ Γ |- A ].
 Proof.
-  intro.
-  destruct X.
-  constructor.
-  exact (redFirstTerm t).
+  induction 1 ; mltt.
 Defined.
+
+#[global] Hint Resolve redFirst : mltt.
 
 Definition redFirstCTerm {Γ t u A} : 
   [ Γ |- t ⇒* u ::: A] ->
   [ Γ |- t ::: A ].
 Proof.
-  intros.
-  destruct X.
-  assumption.
-  exact (redFirstTerm t0).
+  induction 1 ; mltt.
 Defined.
-    
+
+#[global] Hint Resolve redFirstCTerm : mltt.
+
 Definition redFirstC {Γ A B} : 
   [ Γ |- A ⇒* B ] ->
   [ Γ |- A ].
 Proof.
-  intro.
-  destruct X.
-  assumption.
-  exact (redFirst t).
+  induction 1 ; mltt.
 Defined.
 
-Definition redFirstCWFTerm {Γ t u A} : 
+#[global] Hint Resolve redFirstC : mltt.
+
+(*Removed the next two lemmas, as they are just projections…*)
+
+(* Definition redFirstCWFTerm {Γ t u A} : 
   [ Γ |- t :⇒*: u ::: A] ->
   [ Γ |- t ::: A ].
 Proof.
-  intros.
-  destruct X.
-  now eapply redFirstCTerm.
-Defined.
-    
-Definition redFirstCWF {Γ A B} : 
+  now intros [].
+Defined. *)
+
+(* Definition redFirstCWF {Γ A B} : 
   [ Γ |- A :⇒*: B ] ->
   [ Γ |- A ].
 Proof.
-  intro.
-  destruct X.
-  now eapply redFirstC.
-Defined.
+  now intros [].
+Defined. *)
 
 
